From20To30/FunCtx.v
@@ -1,0 +1,300 @@
+From Coq Require Import String ZArith Eqdep_dec.
+
+From Vyper Require Import Config Calldag L10.Base.
+From Vyper Require L20.AST L30.AST L20.Interpret L30.Interpret.
+
+From Vyper.From20To30 Require Import Translate Callset.
+
+(* This might be easier with monads. *)
+Fixpoint alist_maybe_map {Key Value Value' Err: Type}
+                         (KeyEqDec: forall x y: Key, {x = y} + {x <> y})
+                         (a: list (Key * Value)) (f: Value -> Err + Value')
+{struct a}
+: Err + list (Key * Value')
+:= match a with
+   | nil => inr nil
+   | cons (k, v) t =>
+      match f v with
+      | inl err => inl err
+      | inr fv =>
+          match alist_maybe_map KeyEqDec t f with
+          | inl err => inl err
+          | inr mt => inr (cons (k, fv) mt)
+          end
+      end
+   end.
+
+Lemma alist_maybe_map_ok {Key Value Value' Err: Type}
+                         {KeyEqDec: forall x y: Key, {x = y} + {x <> y}}
+                         {a: list (Key * Value)}
+                         {a': list (Key * Value')}
+                         {f: Value -> Err + Value'}
+                         (E: alist_maybe_map KeyEqDec a f = inr a')
+                         (key: Key):
+  match Map.alist_lookup KeyEqDec a key with
+  | Some v =>
+      match f v with
+      | inl _ => False
+      | inr fv => Map.alist_lookup KeyEqDec a' key = Some fv
+      end
+  | None => Map.alist_lookup KeyEqDec a' key =None
+  end.
+Proof.
+revert a' E.
+induction a as [|(k, v)]; intros. { cbn in *. inversion E. now subst. }
+cbn in *.
+remember (KeyEqDec key k) as key_k.
+destruct key_k.
+{
+  destruct (f v). { discriminate. }
+  subst.
+  destruct (alist_maybe_map KeyEqDec a f). { discriminate. }
+  inversion E. subst. cbn.
+  now destruct (KeyEqDec k k).
+}
+destruct (f v). { discriminate. }
+subst.
+destruct (alist_maybe_map KeyEqDec a f). { discriminate. }
+inversion E. subst. cbn.
+rewrite<- Heqkey_k.
+now apply IHa.
+Qed.
+
+Definition map_maybe_map {Key Err: Type} {KeyEqDec: forall x y: Key, {x = y} + {x <> y}}
+                         {Value: Type}
+                         {M: Type}
+                         {MapImpl: Map.class KeyEqDec Value M}
+                         {Value': Type} {M': Type} {MapImpl': Map.class KeyEqDec Value' M'}
+                         (m: M)  (f: Value -> Err + Value')
+: Err + M'
+:= match alist_maybe_map KeyEqDec (Map.items m) f with
+   | inl err => inl err
+   | inr m' => inr (Map.of_alist m')
+   end.
+
+Lemma map_maybe_map_ok {Key Err: Type} {KeyEqDec: forall x y: Key, {x = y} + {x <> y}}
+                       {Value: Type}
+                       {M: Type}
+                       {MapImpl: Map.class KeyEqDec Value M}
+                       {Value': Type} {M': Type} {MapImpl': Map.class KeyEqDec Value' M'}
+                       {m: M}
+                       {f: Value -> Err + Value'}
+                       {m': M'}
+                       (E: map_maybe_map m f = inr m')
+                       (key: Key):
+  match Map.lookup m key with
+  | Some v =>
+      match f v with
+      | inl _ => False
+      | inr fv => Map.lookup m' key = Some fv
+      end
+  | None => Map.lookup m' key =None
+  end.
+Proof.
+unfold map_maybe_map in E.
+remember (alist_maybe_map KeyEqDec (Map.items m) f) as a'.
+destruct a'. { discriminate. }
+assert (L := alist_maybe_map_ok (eq_sym Heqa') key).
+rewrite Map.items_ok.
+destruct (Map.alist_lookup KeyEqDec (Map.items m) key); inversion E; subst.
+{
+  destruct (f v). { easy. }
+  now rewrite Map.of_alist_ok.
+}
+now rewrite Map.of_alist_ok.
+Qed.
+
+Local Lemma translate_calldag_depthmap_ok {C: VyperConfig}
+                                          (name: string)
+                                          (cd: L20.Descend.calldag)
+                                          (d: string_map L30.AST.decl):
+   let _ := string_map_impl in
+   forall E: map_maybe_map (cd_decls cd) translate_decl = inr d,
+     match Map.lookup d name with
+     | Some decl =>
+         match cd_depthmap cd name with
+         | Some x =>
+             let _ := string_set_impl in
+             FSet.for_all (Callset.decl_callset decl)
+               (fun callee : string =>
+                match cd_depthmap cd callee with
+                | Some y => y <? x
+                | None => false
+                end) = true
+         | None => False
+         end
+     | None => True
+     end.
+Proof.
+intros.
+remember (Map.lookup d name) as m.
+destruct m. 2:trivial.
+assert (D := cd_depthmap_ok cd name).
+assert (F := map_maybe_map_ok E name).
+destruct (Map.lookup (cd_decls cd) name). 2:{ now rewrite F in Heqm. }
+destruct (cd_depthmap cd name). 2:assumption.
+rewrite FSet.for_all_ok. rewrite FSet.for_all_ok in D.
+intros x H.
+remember (translate_decl d1) as d30.
+destruct d30. { contradiction. }
+rewrite<- Heqm in F. inversion F; subst.
+rewrite (callset_translate_decl _ _ (eq_sym Heqd30)) in H.
+apply (D x H).
+Qed.
+
+Definition translate_calldag {C: VyperConfig} (cd: L20.Descend.calldag)
+: string + L30.Descend.calldag
+:= let _ := string_map_impl in
+   match map_maybe_map (cd_decls cd) translate_decl as cd' return _ = cd' -> _ with
+   | inl err => fun _ => inl err
+   | inr d => fun E => inr
+     {| cd_decls := d
+      ; cd_depthmap := cd_depthmap cd
+      ; cd_depthmap_ok name := translate_calldag_depthmap_ok name cd d E
+     |}
+   end eq_refl.
+
+(***************************************************************************************************)
+
+Section FunCtx.
+  Context {C: VyperConfig}
+          {bound: nat}
+          {cd20: L20.Descend.calldag}
+          (fc: fun_ctx cd20 bound)
+          {cd30: L30.Descend.calldag}
+          (ok: translate_calldag cd20 = inr cd30).
+
+  Lemma translate_fun_ctx_depthmap (name: string):
+    cd_depthmap cd30 name
+     =
+    cd_depthmap cd20 name.
+  Proof.
+  destruct cd20.
+  unfold translate_calldag in ok.
+  cbn in *.
+  remember (fun d (E : map_maybe_map cd_decls translate_decl = inr d) =>
+         inr
+           {|
+           cd_decls := d;
+           cd_depthmap := cd_depthmap;
+           cd_depthmap_ok := fun name : string =>
+                             translate_calldag_depthmap_ok name
+                               {|
+                               cd_decls := cd_decls;
+                               cd_depthmap := cd_depthmap;
+                               cd_depthmap_ok := cd_depthmap_ok |} d E |}) as good_branch.
+  assert (K: forall (d30: string_map L30.AST.decl)
+                    (E: map_maybe_map cd_decls translate_decl = inr d30),
+               good_branch d30 E = inr cd30 
+                ->
+               Calldag.cd_depthmap cd30 name = cd_depthmap name).
+  {
+    intros. subst.
+    inversion H. now subst.
+  }
+  clear Heqgood_branch.
+  destruct (map_maybe_map cd_decls translate_decl) as [|d30]. { discriminate. }
+  apply (K d30 eq_refl ok).
+  Qed.
+
+  Lemma translate_fun_ctx_declmap (name: string):
+    match cd_declmap cd20 name with
+    | Some d => Some (translate_decl d)
+    | None => None
+    end
+     =
+    match cd_declmap cd30 name with
+    | Some d => Some (inr d)
+    | None => None
+    end.
+  Proof.
+  destruct cd20.
+  unfold translate_calldag in ok.
+  cbn in *.
+  remember (fun d (E : map_maybe_map cd_decls translate_decl = inr d) =>
+         inr
+           {|
+           cd_decls := d;
+           cd_depthmap := cd_depthmap;
+           cd_depthmap_ok := fun name : string =>
+                             translate_calldag_depthmap_ok name
+                               {|
+                               cd_decls := cd_decls;
+                               cd_depthmap := cd_depthmap;
+                               cd_depthmap_ok := cd_depthmap_ok |} d E |}) as good_branch.
+  unfold cd_declmap. cbn.
+  assert (K: forall (d30: string_map L30.AST.decl)
+                    (E: map_maybe_map cd_decls translate_decl = inr d30),
+               good_branch d30 E = inr cd30 
+                ->
+               let _ := string_map_impl in
+               match Map.lookup cd_decls name with
+               | Some d => Some (translate_decl d)
+               | None => None
+               end = match Map.lookup (Calldag.cd_decls cd30) name with
+                     | Some d => Some (inr d)
+                     | None => None
+                     end).
+  {
+    intros. subst.
+    inversion H. subst.
+    cbn.
+    clear H ok.
+    assert (M := map_maybe_map_ok E name).
+    destruct (Map.lookup cd_decls name). 2:{ now destruct Map.lookup. }
+    destruct (translate_decl d). { contradiction. }
+    (* why rewrite M doesn't work? *)
+    destruct Map.lookup. { now inversion M. }
+    discriminate.
+  }
+  clear Heqgood_branch.
+  destruct (map_maybe_map cd_decls translate_decl) as [|d30]. { discriminate. }
+  apply (K d30 eq_refl ok).
+  Qed.
+
+  Local Lemma translate_fun_ctx_fun_decl_helper:
+    cd_declmap cd30 (fun_name fc) <> None.
+  Proof.
+  intro E.
+  assert (Ok := fun_decl_ok fc).
+  assert (M := translate_fun_ctx_declmap (fun_name fc)).
+  rewrite Ok in M.
+  rewrite E in M.
+  discriminate.
+  Qed.
+
+  Definition cached_translated_decl
+  := match cd_declmap cd30 (fun_name fc)
+     as d' return _ = d' -> _
+     with
+     | Some f => fun _ => f
+     | None => fun E =>
+          False_rect _ (translate_fun_ctx_fun_decl_helper E)
+     end eq_refl.
+
+  Local Lemma translate_fun_ctx_decl_ok:
+    cd_declmap cd30 (fun_name fc) 
+     =
+    Some cached_translated_decl.
+  Proof.
+  assert (D := fun_decl_ok fc).
+  unfold cached_translated_decl.
+  remember translate_fun_ctx_fun_decl_helper as foo. clear Heqfoo. revert foo.
+  destruct (cd_declmap cd30 (fun_name fc)). { trivial. }
+  intro. contradiction.
+  Qed.
+
+  Definition translate_fun_ctx
+  : fun_ctx cd30 bound
+  := let name := fun_name fc in
+     {| fun_name := name
+      ; fun_depth := fun_depth fc
+      ; fun_depth_ok :=
+          eq_trans (translate_fun_ctx_depthmap name)
+                   (fun_depth_ok fc)
+      ; fun_decl := cached_translated_decl
+      ; fun_decl_ok := translate_fun_ctx_decl_ok
+      ; fun_bound_ok := fun_bound_ok fc
+     |}.
+
+End FunCtx.
