L30/Descend.v
@@ -43,6 +43,7 @@ assert(HasName: let _ := string_set_impl in FSet.has (decl_callset this_decl) na
 }
 clear CallOk. cbn in HasName.
 assert (K := cd_depthmap_ok cd this_fun_name).
+unfold cd_declmap in this_decl_ok.
 rewrite this_decl_ok in K.
 rewrite current_fun_depth_ok in K.
 cbn in K.
@@ -64,6 +65,7 @@ Local Lemma fun_ctx_descend_helper {cd: calldag}
   cd_depthmap cd name <> None.
 Proof.
 assert (D := cd_depthmap_ok cd name).
+unfold cd_declmap in *.
 rewrite Edecl in D.
 intro H.
 rewrite H in D.
